Proof Without Words with gganimate
================

Example 1:
----------

$$ \\sum\_{i = 1}^n(2i - 1) = n^2 $$
 The animated version of the proof is show below:

![](figures/sum_of_odds.gif)

Example 2:
----------

1<sup>3</sup> + 2<sup>3</sup> + … + (*n* − 1)<sup>3</sup> + *n*<sup>3</sup> = (1 + 2 + … + *n*)<sup>2</sup>
 The animated version of the proof is shown below:

![](figures/sum_of_cubes.gif)

Example 3
---------

$$ \\frac{1}{2^2} + \\frac{1}{2^4} + \\frac{1}{2^6} + \\frac{1}{2^8} + \\ldots = \\frac{1}{3} $$
 ![](figures/infinite_series_1.gif)

Example 4
---------

![](figures/pythagoras_theorem.gif)
